<?xml version="1.0"?>
<?xml-stylesheet type="text/xsl" href="human.xsl"?>
<!-- $Rev: 1399 $ -->
<!-- $Date: 2008-08-08 12:12:15 +0100 (Fri, 08 Aug 2008) $ -->
<!-- $Author: RogerHyam $ -->
<rdf:RDF xml:base="http://rs.tdwg.org/ontology/voc/Institution" xmlns="http://rs.tdwg.org/ontology/voc/Institution#" xmlns:dc="http://purl.org/dc/elements/1.1/" xmlns:dcterms="http://purl.org/dc/terms/" xmlns:owl="http://www.w3.org/2002/07/owl#" xmlns:rdf="http://www.w3.org/1999/02/22-rdf-syntax-ns#" xmlns:rdfs="http://www.w3.org/2000/01/rdf-schema#" xmlns:tbase="http://rs.tdwg.org/ontology/Base#" xmlns:tcom="http://rs.tdwg.org/ontology/voc/Common#" xmlns:tcore="http://rs.tdwg.org/ontology/Core#" xmlns:tinst="http://rs.tdwg.org/ontology/voc/Institution#" xmlns:titype="http://rs.tdwg.org/ontology/voc/InstitutionType#">
	<owl:Ontology rdf:about="http://rs.tdwg.org/ontology/voc/Institution">
		<dc:title>TDWG Institution LSID Ontology</dc:title>
		<dc:creator>Markus DÃ¶ring</dc:creator>
		<dc:publisher>TDWG Biodiversity Information Standards - NCD subgroup</dc:publisher>
        <dcterms:issued>2007-03-08</dcterms:issued>
		<dcterms:modified>$Date: 2008-08-08 12:12:15 +0100 (Fri, 08 Aug 2008) $</dcterms:modified>
		<dc:description>Ontology describing the metadata returned for LSIDs that are used for institutional records. i.e. public or private institutions such as universities, museums, gardens, research
         labs, etc. 
      </dc:description>
		<owl:versionInfo>0.7 - [SVN $Rev: 1399 $]</owl:versionInfo>
		<rdfs:comment rdf:parseType="Literal">
        The name and subname of an organisation is part of the Contact vCard details.
        The preferred name/title for the organisation should also be given as a DC:TITLE property
      </rdfs:comment>
	</owl:Ontology>
	<!-- *************************************************
					I N S T I T U T I O N
 		**************************************************** -->
	<!-- Institution -->
	<owl:Class rdf:ID="Institution">
		<rdfs:label>Institution</rdfs:label>
		<rdfs:comment>A public or private institution</rdfs:comment>
		<rdfs:subClassOf rdf:resource="http://rs.tdwg.org/ontology/Base#BaseThing"/>
		<rdfs:isDefinedBy rdf:resource="http://rs.tdwg.org/ontology/voc/Institution"/>
	</owl:Class>
	<owl:DatatypeProperty rdf:ID="institutionId">
		<rdfs:label>Institution Identifier</rdfs:label>
		<rdfs:comment>The URI (LSID or URL) of the the institution. In RDF this will be used as URI of the collection resource.</rdfs:comment>
		<rdfs:domain rdf:resource="#Collection"/>
		<rdfs:range rdf:resource="http://www.w3.org/2001/XMLSchema#string"/>
		<rdfs:isDefinedBy rdf:resource="http://rs.tdwg.org/ontology/voc/Collection"/>
	</owl:DatatypeProperty>
	<owl:ObjectProperty rdf:ID="hasContact">
		<rdfs:label>hasContact</rdfs:label>
		<rdfs:comment>A link to contact information (such as postal address, email address and phone number) for this institution.</rdfs:comment>
		<rdfs:domain rdf:resource="#Institution"/>
		<rdfs:range rdf:resource="http://rs.tdwg.org/ontology/voc/ContactDetails#ContactDetails"/>
		<rdfs:isDefinedBy rdf:resource="http://rs.tdwg.org/ontology/voc/Institution"/>
	</owl:ObjectProperty>
	<owl:ObjectProperty rdf:ID="isPartOfInstitution">
		<rdfs:label>Parent Institution or Network</rdfs:label>
		<rdfs:comment>Name, acronym or coden of parent institution or network(s)</rdfs:comment>
		<rdfs:domain rdf:resource="#Institution"/>
		<rdfs:range rdf:resource="#Institution"/>
		<rdfs:isDefinedBy rdf:resource="http://rs.tdwg.org/ontology/voc/Institution"/>
	</owl:ObjectProperty>
	<owl:ObjectProperty rdf:ID="institutionType">
		<rdfs:label>Institution Type</rdfs:label>
		<rdfs:comment>Picklist keyword describing the primary activity or purpose of an organization or entity that holds or uses collections.</rdfs:comment>
		<rdfs:domain rdf:resource="#Institution"/>
		<rdfs:range rdf:resource="http://rs.tdwg.org/ontology/voc/InstitutionType#InstitutionTypeTerm"/>
		<rdfs:isDefinedBy rdf:resource="http://rs.tdwg.org/ontology/voc/Institution"/>
	</owl:ObjectProperty>
	<owl:ObjectProperty rdf:ID="alternativeId">
		<rdfs:label>Alternative ID</rdfs:label>
		<rdfs:comment>Alternative identifier for the institution indicating the source, e.g. Index Herbariorum.</rdfs:comment>
		<rdfs:domain rdf:resource="#Institution"/>
		<rdfs:range rdf:resource="http://rs.tdwg.org/ontology/voc/TermWithSource"/>
		<rdfs:isDefinedBy rdf:resource="http://rs.tdwg.org/ontology/voc/Institution"/>
	</owl:ObjectProperty>
	<owl:ObjectProperty rdf:ID="acronymOrCoden">
		<rdfs:label>Acronym Or Coden</rdfs:label>
		<rdfs:comment>Acronym, coden or initialism by which the institution is generally known indicating the source, e.g. Index Herbariorum.</rdfs:comment>
		<rdfs:domain rdf:resource="#Institution"/>
		<rdfs:range rdf:resource="http://rs.tdwg.org/ontology/voc/TermWithSource"/>
		<rdfs:isDefinedBy rdf:resource="http://rs.tdwg.org/ontology/voc/Institution"/>
	</owl:ObjectProperty>
	<owl:ObjectProperty rdf:ID="hasCollection">
		<rdfs:label>hasCollection</rdfs:label>
		<rdfs:comment>A link to a collection description.</rdfs:comment>
		<rdfs:domain rdf:resource="#Institution"/>
		<rdfs:range rdf:resource="http://rs.tdwg.org/ontology/voc/Collection#Collection"/>
		<rdfs:isDefinedBy rdf:resource="http://rs.tdwg.org/ontology/voc/Institution"/>
	</owl:ObjectProperty>
</rdf:RDF>
