<?xml version="1.0" encoding="UTF-8"?>
<?xml-stylesheet type="text/xsl" href="human.xsl"?>
<!-- $Rev: 1294 $ -->
<!-- $Date: 2007-08-15 14:05:50 +0100 (Wed, 15 Aug 2007) $ -->
<!-- $Author: MarkusDoering $ -->

<rdf:RDF xmlns:rdf="http://www.w3.org/1999/02/22-rdf-syntax-ns#"
   xmlns:rdfs="http://www.w3.org/2000/01/rdf-schema#" xmlns:owl="http://www.w3.org/2002/07/owl#"
   xmlns:dc="http://purl.org/dc/elements/1.1/" xmlns:dcterms="http://purl.org/dc/terms/"
   xmlns:tbase="http://rs.tdwg.org/ontology/Base#" xmlns:tcore="http://rs.tdwg.org/ontology/Core#"
   xmlns:tcom="http://rs.tdwg.org/ontology/voc/Common#"
   xmlns="http://rs.tdwg.org/ontology/voc/Specimen#"
   xmlns:tsp="http://rs.tdwg.org/ontology/voc/Specimen#"
   xml:base="http://rs.tdwg.org/ontology/voc/Specimen">
   <owl:Ontology rdf:about="http://rs.tdwg.org/ontology/voc/Specimen">
      <dc:title>TDWG Specimen LSID Ontology</dc:title>
      <dc:creator>Roger Hyam</dc:creator>
      <dc:publisher>TDWG Biodiversity Information Standards</dc:publisher>
      <dcterms:issued>2007-01-30</dcterms:issued>
      <dcterms:modified>$Date: 2007-08-15 14:05:50 +0100 (Wed, 15 Aug 2007) $</dcterms:modified>
      <dc:description>Ontology describing the metadata returned for LSIDs that are used for specimen
         records. </dc:description>

      <owl:versionInfo>0.2 - [SVN $Rev: 1294 $]</owl:versionInfo>

      <rdfs:comment rdf:parseType="Literal"> *** This vocabulary has been superseded by the
         TaxonOccurrence vocabulary (http://rs.tdwg.org/ontology/voc/TaxonOccurrence) Read more
         about this on the associated wiki page.****
         http://wiki.tdwg.org/twiki/bin/view/TAG/TaxonOccurrenceLsidVoc This ontology is designed to
         represent records of specimens. Note that it contains informations specific to the
         specimen. Data about the occurrence of a taxon in the wild that this specimen was taken
         from should be given in a OccurrenceRecord object in the voucherFor property.</rdfs:comment>

   </owl:Ontology>
   <!-- *************************************************
					S P E C I M E N  
 		**************************************************** -->
   <!-- Specimen -->
   <owl:Class rdf:ID="Specimen">
      <rdfs:label>Specimen</rdfs:label>
      <rdfs:comment>A biological specimen.</rdfs:comment>
      <rdfs:subClassOf rdf:resource="http://rs.tdwg.org/ontology/Base#BaseThing"/>
      <rdfs:isDefinedBy rdf:resource="http://rs.tdwg.org/ontology/voc/Specimen"/>
   </owl:Class>

   <!-- Specimen::isVoucherFor -->
   <owl:ObjectProperty rdf:ID="isVoucherFor">
      <rdfs:label>Is Voucher For</rdfs:label>
      <rdfs:comment>This specimen is a voucher for another record of some kind e.g. an
         OccurrenceRecord</rdfs:comment>
      <rdfs:domain rdf:resource="#Specimen"/>
      <rdfs:range rdf:resource="http://rs.tdwg.org/ontology/voc/OccurrenceRecord#OccurrenceRecord"/>
      <rdfs:isDefinedBy rdf:resource="http://rs.tdwg.org/ontology/voc/Specimen"/>
   </owl:ObjectProperty>

   <!-- Specimen::derivedFrom -->
   <owl:ObjectProperty rdf:ID="derivedFrom">
      <rdfs:label>Derived From</rdfs:label>
      <rdfs:comment>This Specimen has been derived from another occurrence record following some
         procedure that may be documented by the procedure property.</rdfs:comment>
      <rdfs:domain rdf:resource="#Specimen"/>
      <rdfs:range rdf:resource="http://rs.tdwg.org/ontology/voc/Specimen#Specimen"/>
      <rdfs:isDefinedBy rdf:resource="http://rs.tdwg.org/ontology/voc/Specimen"/>
   </owl:ObjectProperty>

   <!-- Specimen::procedure -->
   <owl:ObjectProperty rdf:ID="procedure">
      <rdfs:label>Procedure</rdfs:label>
      <rdfs:comment>The procedure followed that generated this object perhaps by derivation from
         another specimen.</rdfs:comment>
      <rdfs:domain rdf:resource="#Specimen"/>
      <rdfs:range rdf:resource="http://rs.tdwg.org/ontology/voc/Procedure#Procedure"/>
      <rdfs:isDefinedBy rdf:resource="http://rs.tdwg.org/ontology/voc/Specimen"/>
      <dc:relation rdf:resource="http://rs.tdwg.org/ontology/voc/Specimen#procedureDescriptor"/>
   </owl:ObjectProperty>

   <!-- Specimen::procedureDescriptor -->
   <owl:DatatypeProperty rdf:ID="procedureDescriptor">
      <rdfs:label>Procedure Descriptor</rdfs:label>
      <rdfs:comment>A string description of the procedure employed in generating this specimen. This
         may be interpreted in combination with and qualifying the procedure property.</rdfs:comment>
      <rdfs:domain rdf:resource="#Specimen"/>
      <rdfs:range rdf:resource="http://www.w3.org/2001/XMLSchema#string"/>
      <rdfs:isDefinedBy rdf:resource="http://rs.tdwg.org/ontology/voc/Specimen"/>
      <dc:relation rdf:resource="http://rs.tdwg.org/ontology/voc/Specimen#procedure"/>
   </owl:DatatypeProperty>


   <!-- Specimen::collector -->
   <owl:DatatypeProperty rdf:ID="collector">
      <rdfs:label>Collector</rdfs:label>
      <rdfs:comment>The name(s) of the collector(s) of the specimen. These may be normalised out in
         the collectorTeam property.</rdfs:comment>
      <rdfs:domain rdf:resource="#Specimen"/>
      <rdfs:range rdf:resource="http://www.w3.org/2001/XMLSchema#string"/>
      <rdfs:isDefinedBy rdf:resource="http://rs.tdwg.org/ontology/voc/Specimen"/>
      <tcom:darwinCoreEquivalence>Core:Collector</tcom:darwinCoreEquivalence>
      <dc:relation rdf:resource="http://rs.tdwg.org/ontology/voc/Specimen#collectorTeam"/>
   </owl:DatatypeProperty>

   <!-- Specimen::collectorTeam -->
   <owl:ObjectProperty rdf:ID="collectorTeam">
      <rdfs:label>Collector Team</rdfs:label>
      <rdfs:comment>A breakdown of the collectors of the specimen. An expansion of the information
         given in the collector property.</rdfs:comment>
      <rdfs:domain rdf:resource="#Specimen"/>
      <rdfs:range rdf:resource="http://rs.tdwg.org/ontology/voc/Team#Team"/>
      <rdfs:isDefinedBy rdf:resource="http://rs.tdwg.org/ontology/voc/Specimen"/>
      <dc:relation rdf:resource="http://rs.tdwg.org/ontology/voc/Specimen#collector"/>
   </owl:ObjectProperty>

   <!-- Specimen::collectorsFieldNumber -->
   <owl:DatatypeProperty rdf:ID="collectorsFieldNumber">
      <rdfs:label>Collectors Field Number</rdfs:label>
      <rdfs:comment>The identifier issued for the specimen by the collector at the time of
         collection.</rdfs:comment>
      <rdfs:domain rdf:resource="#Specimen"/>
      <rdfs:range rdf:resource="http://www.w3.org/2001/XMLSchema#string"/>
      <rdfs:isDefinedBy rdf:resource="http://rs.tdwg.org/ontology/voc/Specimen"/>
      <tcom:darwinCoreEquivalence>CuratorialExtension:CollectorNumber</tcom:darwinCoreEquivalence>
      <tcom:abcdEquivalence>CollectorsFieldNumber</tcom:abcdEquivalence>
   </owl:DatatypeProperty>

   <!-- Specimen::collectorsBatchNumber -->
   <owl:DatatypeProperty rdf:ID="collectorsBatchNumber">
      <rdfs:label>Collector's Batch Number</rdfs:label>
      <rdfs:comment>An identifying string applied to a set of objects or observations resulting from
         a single collecting event.</rdfs:comment>
      <rdfs:domain rdf:resource="#Specimen"/>
      <rdfs:range rdf:resource="http://www.w3.org/2001/XMLSchema#string"/>
      <rdfs:isDefinedBy rdf:resource="http://rs.tdwg.org/ontology/voc/Specimen"/>
      <tcom:darwinCoreEquivalence>CuratorialExtension:FieldNumber</tcom:darwinCoreEquivalence>
      <tcom:abcdEquivalence>CollectorsFieldNumber</tcom:abcdEquivalence>
   </owl:DatatypeProperty>

   <!-- Specimen::kindOfSpecimen -->
   <owl:ObjectProperty rdf:ID="kindOfSpecimen">
      <rdfs:label>kindOfSpecimen</rdfs:label>
      <rdfs:comment>The kind of object this specimen is e.g. herbarium, fossil, living, moving
         image, sound recording etc. This property may be repeated, for example a specimen may be a
         herbarium specimen and also a moss packet. In addition to indicating the specimen kind with
         this flag implementers may choose to subclass Specimen. It is recommended that even if the
         Specimen class is subclassed and specialised kinds of specimens added to the vocabulary the
         same basic KindOfSpecimen terms are always included to enable naive clients to interpret
         the object. A graphical client may have a small number of icons to display next to well
         known specimen types for example.</rdfs:comment>
      <rdfs:domain rdf:resource="#Specimen"/>
      <rdfs:range rdf:resource="http://rs.tdwg.org/ontology/voc/Specimen#KindOfSpecimenTerm"/>
      <rdfs:isDefinedBy rdf:resource="http://rs.tdwg.org/ontology/voc/Specimen"/>
      <tcom:darwinCoreEquivalence>Core:BasisOfRecord - but note that this is only for kinds of
         physical voucher object not observations.</tcom:darwinCoreEquivalence>
      <tcom:abcdEquivalence>BasisOfRecord and KindOfUnit but note that this is only for kinds of
         physical voucher object not observations.</tcom:abcdEquivalence>
      <dc:relation rdf:resource="http://rs.tdwg.org/ontology/voc/Specimen#kindOfSpecimenString"/>
   </owl:ObjectProperty>

   <!-- Specimen::kindOfSpecimenString -->
   <owl:DatatypeProperty rdf:ID="kindOfSpecimenString">
      <rdfs:label>kindOfSpecimenString</rdfs:label>
      <rdfs:comment>This is a human readable account of the kind of specimen given by the
         kindOfSpecimen property. It allows for use of descriptive terms that may not be available
         from a controlled vocabulary. Wherever possible the kindOfSpecimen should be used as well
         as this property. </rdfs:comment>
      <rdfs:domain rdf:resource="#Specimen"/>
      <rdfs:range rdf:resource="http://www.w3.org/2001/XMLSchema#string"/>
      <rdfs:isDefinedBy rdf:resource="http://rs.tdwg.org/ontology/voc/Specimen"/>
      <tcom:darwinCoreEquivalence>Core:BasisOfRecord - but note that this is only for kinds of
         physical voucher object not observations.</tcom:darwinCoreEquivalence>
      <tcom:abcdEquivalence>BasisOfRecord and KindOfUnit but note that this is only for kinds of
         physical voucher object not observations.</tcom:abcdEquivalence>
      <dc:relation rdf:resource="http://rs.tdwg.org/ontology/voc/Specimen#kindOfSpecimen"/>
   </owl:DatatypeProperty>

   <!-- Specimen::hostCollection -->
   <owl:ObjectProperty rdf:ID="hostCollection">
      <rdfs:label>Host Collection</rdfs:label>
      <rdfs:comment>A link to the collection that hosts this specimen. The collection will contain
         details of the collection code and host institution/organisation.</rdfs:comment>
      <rdfs:domain rdf:resource="#Specimen"/>
      <rdfs:range rdf:resource="http://rs.tdwg.org/ontology/voc/Collection#Collection"/>
      <rdfs:isDefinedBy rdf:resource="http://rs.tdwg.org/ontology/voc/Specimen"/>
      <dc:relation rdf:resource="http://rs.tdwg.org/ontology/voc/Specimen#hostCollectionString"/>
   </owl:ObjectProperty>

   <!-- Specimen::hostCollectionString -->
   <owl:DatatypeProperty rdf:ID="hostCollectionString">
      <rdfs:label>Host Collection String</rdfs:label>
      <rdfs:comment>A string representation of the collection hosting this specimen. May include the
         collection and institution codes. May be normalised in the hostCollection property.</rdfs:comment>
      <rdfs:domain rdf:resource="#Specimen"/>
      <rdfs:range rdf:resource="http://www.w3.org/2001/XMLSchema#string"/>
      <rdfs:isDefinedBy rdf:resource="http://rs.tdwg.org/ontology/voc/Specimen"/>
      <tcom:darwinCoreEquivalence>Core:InstitutionCode and Core:CollectionCode</tcom:darwinCoreEquivalence>
      <tcom:abcdEquivalence>SourceInstitutionID</tcom:abcdEquivalence>
      <dc:relation rdf:resource="http://rs.tdwg.org/ontology/voc/Specimen#hostCollection"/>
   </owl:DatatypeProperty>

   <!-- Specimen::specimenID -->
   <owl:DatatypeProperty rdf:ID="specimenID">
      <rdfs:label>Specimen ID</rdfs:label>
      <rdfs:comment>The identifier used for this specimen within the scope of the collection. e.g.
         catalogue number. This should be the preferred identifier. Alternative identifiers, such as
         barcodes, can be given using the dc:identifier property. </rdfs:comment>
      <rdfs:domain rdf:resource="#Specimen"/>
      <rdfs:range rdf:resource="http://www.w3.org/2001/XMLSchema#string"/>
      <rdfs:isDefinedBy rdf:resource="http://rs.tdwg.org/ontology/voc/Specimen"/>
      <tcom:darwinCoreEquivalence>CatalogNumber</tcom:darwinCoreEquivalence>
      <tcom:abcdEquivalence>UnitID</tcom:abcdEquivalence>
   </owl:DatatypeProperty>

   <!-- Specimen::verbatimLabelText -->
   <owl:DatatypeProperty rdf:ID="verbatimLabelText">
      <rdfs:label>Verbatim Label Text</rdfs:label>
      <rdfs:comment>The text as it occurs on the label of the specimen.</rdfs:comment>
      <rdfs:domain rdf:resource="#Specimen"/>
      <rdfs:range rdf:resource="http://www.w3.org/2001/XMLSchema#string"/>
      <rdfs:isDefinedBy rdf:resource="http://rs.tdwg.org/ontology/voc/Specimen"/>
   </owl:DatatypeProperty>

   <!-- Specimen::digitalRepresentation -->
   <owl:ObjectProperty rdf:ID="digitalRepresentation">
      <rdfs:label>Digital Representation</rdfs:label>
      <rdfs:comment>A link to a digital representation of this specimen. e.g. an image of the
         herbarium specimen. If the specimen is an actual digital object (such as a sound recording)
         and available via the getData() call of the LSID then this property could be ambiguous in
         which case the following procedure should be followed. If the LSID getData() call maps to
         an HTTP GET call on a stable URI then that URI could be included here. This would enable
         non LSID aware clients to access the data. If the getData() call does not map in this way
         then this property should be omitted. If there are alternative digital representations of
         the object available (e.g. a sound recording in another format) then the
         DublinCore::hasFormat property should be used. </rdfs:comment>
      <rdfs:domain rdf:resource="#Specimen"/>
      <rdfs:isDefinedBy rdf:resource="http://rs.tdwg.org/ontology/voc/Specimen"/>
      <dc:relation rdf:resource="http://rs.tdwg.org/ontology/voc/Specimen#hostCollectionString"/>
   </owl:ObjectProperty>

   <!-- Specimen::typeStatusString -->
   <owl:DatatypeProperty rdf:ID="typeStatusString">
      <rdfs:label>Type Status String</rdfs:label>
      <rdfs:comment>A list of one or more nomenclatural types (including type status and typified
         taxonomic name) represented by the object. Example: "holotype of Ctenomys sociabilis.
         Pearson O. P., and M. I. Christie. 1985. Historia Natural, 5(37):388" </rdfs:comment>
      <rdfs:domain rdf:resource="#Specimen"/>
      <rdfs:range rdf:resource="http://www.w3.org/2001/XMLSchema#string"/>
      <rdfs:isDefinedBy rdf:resource="http://rs.tdwg.org/ontology/voc/Specimen"/>
      <dc:relation rdf:resource="http://rs.tdwg.org/ontology/voc/Specimen#typeStatus"/>
      <tcom:darwinCoreEquivalence>Curatorial::TypeStatus</tcom:darwinCoreEquivalence>
   </owl:DatatypeProperty>

   <!-- Specimen::typeStatus ... indication of the type of type this specimen is -->
   <owl:ObjectProperty rdf:ID="typeStatus">
      <rdfs:label>Type Status String</rdfs:label>
      <rdfs:comment>The type of type specimen this specimen is.</rdfs:comment>
      <rdfs:domain rdf:resource="#Specimen"/>
      <rdfs:range rdf:resource="http://rs.tdwg.org/ontology/voc/TaxonName#NomenclaturalTypeTypeTerm"/>
      <rdfs:isDefinedBy rdf:resource="http://rs.tdwg.org/ontology/voc/Specimen"/>
      <dc:relation rdf:resource="http://rs.tdwg.org/ontology/voc/Specimen#typeStatusString"/>
      <tcom:darwinCoreEquivalence>Curatorial::TypeStatus - but as a controlled vocabulary rather
         than a string.</tcom:darwinCoreEquivalence>
   </owl:ObjectProperty>

   <!-- Specimen::typeForName .. a name for which this is the type -->
   <owl:ObjectProperty rdf:ID="typeForName">
      <rdfs:label>Type For Name</rdfs:label>
      <rdfs:comment>A name for which this specimen is a type.</rdfs:comment>
      <rdfs:domain rdf:resource="#Specimen"/>
      <rdfs:range rdf:resource="http://rs.tdwg.org/ontology/voc/TaxonName#TaxonName"/>
      <rdfs:isDefinedBy rdf:resource="http://rs.tdwg.org/ontology/voc/Specimen"/>
      <dc:relation rdf:resource="http://rs.tdwg.org/ontology/voc/Specimen#typeStatus"/>
   </owl:ObjectProperty>

   <!-- Specimen::disposition -->
   <owl:DatatypeProperty rdf:ID="disposition">
      <rdfs:label>Disposition</rdfs:label>
      <rdfs:comment>The current disposition of the cataloged item. Examples: "in collection",
         "missing", "voucher elsewhere", "duplicates elsewhere".</rdfs:comment>
      <rdfs:domain rdf:resource="#Specimen"/>
      <rdfs:range rdf:resource="http://www.w3.org/2001/XMLSchema#string"/>
      <rdfs:isDefinedBy rdf:resource="http://rs.tdwg.org/ontology/voc/Specimen"/>
      <tcom:darwinCoreEquivalence>Curatorial::Disposition</tcom:darwinCoreEquivalence>
   </owl:DatatypeProperty>

   <!-- Specimen::individualCount -->
   <owl:DatatypeProperty rdf:ID="individualCount">
      <rdfs:label>Individual Count</rdfs:label>
      <rdfs:comment>The number of individuals present in the lot or container. Not to be used for
         observations - see OccurrenceRecord/value property.</rdfs:comment>
      <rdfs:domain rdf:resource="#Specimen"/>
      <rdfs:range rdf:resource="http://www.w3.org/2001/XMLSchema#string"/>
      <rdfs:isDefinedBy rdf:resource="http://rs.tdwg.org/ontology/voc/Specimen"/>
      <tcom:darwinCoreEquivalence>Curatorial::IndividualCount</tcom:darwinCoreEquivalence>
   </owl:DatatypeProperty>

   <!-- Specimen::verbatimCoordinates -->
   <owl:DatatypeProperty rdf:ID="verbatimCoordinates">
      <rdfs:label>Verbatim Coordinates</rdfs:label>
      <rdfs:comment>A text representation of the coordinate data (Latitude/ Longitude, UTM, TRS,
         etc.) from its original source if it cannot be separated into its component parts. Example:
         "470999 1234300".</rdfs:comment>
      <rdfs:domain rdf:resource="#Specimen"/>
      <rdfs:range rdf:resource="http://www.w3.org/2001/XMLSchema#string"/>
      <rdfs:isDefinedBy rdf:resource="http://rs.tdwg.org/ontology/voc/Specimen"/>
      <tcom:darwinCoreEquivalence>Geospatial:VerbatimCoordinates</tcom:darwinCoreEquivalence>
   </owl:DatatypeProperty>

   <!-- Specimen::verbatimLatitude -->
   <owl:DatatypeProperty rdf:ID="verbatimLatitude">
      <rdfs:label>Verbatim Latitude</rdfs:label>
      <rdfs:comment>A text representation of the Latitude part of the coordinate data from its
         original source. Example: 47d09'99"N</rdfs:comment>
      <rdfs:domain rdf:resource="#Specimen"/>
      <rdfs:range rdf:resource="http://www.w3.org/2001/XMLSchema#string"/>
      <rdfs:isDefinedBy rdf:resource="http://rs.tdwg.org/ontology/voc/Specimen"/>
      <tcom:darwinCoreEquivalence>Geospatial:VerbatimLatitude</tcom:darwinCoreEquivalence>
   </owl:DatatypeProperty>

   <!-- Specimen::verbatimLongitude -->
   <owl:DatatypeProperty rdf:ID="verbatimLongitude">
      <rdfs:label>Verbatim Longitude</rdfs:label>
      <rdfs:comment>A text representation of the Longitude part of the coordinate data from its
         original source. Example: -122.43254</rdfs:comment>
      <rdfs:domain rdf:resource="#Specimen"/>
      <rdfs:range rdf:resource="http://www.w3.org/2001/XMLSchema#string"/>
      <rdfs:isDefinedBy rdf:resource="http://rs.tdwg.org/ontology/voc/Specimen"/>
      <tcom:darwinCoreEquivalence>Geospatial:VerbatimLongitude</tcom:darwinCoreEquivalence>
   </owl:DatatypeProperty>

   <!-- Specimen::verbatimCoordinateSystem -->
   <owl:DatatypeProperty rdf:ID="verbatimCoordinateSystem">
      <rdfs:label>Verbatim Coordinate System</rdfs:label>
      <rdfs:comment>The name of the system in which the verbatim geographic coordinates were
         recorded. Examples: "decimal degrees", "degrees minutes seconds", "degrees decimal
         minutes", "UTM"</rdfs:comment>
      <rdfs:domain rdf:resource="#Specimen"/>
      <rdfs:range rdf:resource="http://www.w3.org/2001/XMLSchema#string"/>
      <rdfs:isDefinedBy rdf:resource="http://rs.tdwg.org/ontology/voc/Specimen"/>
      <tcom:darwinCoreEquivalence>Geospatial:VerbatimCoordinateSystem</tcom:darwinCoreEquivalence>
   </owl:DatatypeProperty>

   <!-- Specimen::verbatimCollectingDate -->
   <owl:DatatypeProperty rdf:ID="verbatimCollectingDate">
      <rdfs:label>Verbatim Collecting Date</rdfs:label>
      <rdfs:comment>The verbatim original representation of the date (and time) information for the
         collecting event as recorded on the specimen or collection catalogue Example: "spring 1910"</rdfs:comment>
      <rdfs:domain rdf:resource="#Specimen"/>
      <rdfs:range rdf:resource="http://www.w3.org/2001/XMLSchema#string"/>
      <rdfs:isDefinedBy rdf:resource="http://rs.tdwg.org/ontology/voc/Specimen"/>
      <tcom:darwinCoreEquivalence>Curatorial:VerbatimCollectingDate</tcom:darwinCoreEquivalence>
   </owl:DatatypeProperty>

   <!-- Specimen::verbatimElevation -->
   <owl:DatatypeProperty rdf:ID="verbatimElevation">
      <rdfs:label>Verbatim Elevation</rdfs:label>
      <rdfs:comment> A text representation of the altitude in its original format as on the specimen
         or in the collection catalogue. Example: "1000+- meters".</rdfs:comment>
      <rdfs:domain rdf:resource="#Specimen"/>
      <rdfs:range rdf:resource="http://www.w3.org/2001/XMLSchema#string"/>
      <rdfs:isDefinedBy rdf:resource="http://rs.tdwg.org/ontology/voc/Specimen"/>
      <tcom:darwinCoreEquivalence>Curatorial:VerbatimElevation</tcom:darwinCoreEquivalence>
   </owl:DatatypeProperty>

   <!-- Specimen::verbatimDepth -->
   <owl:DatatypeProperty rdf:ID="verbatimDepth">
      <rdfs:label>Verbatim Depth</rdfs:label>
      <rdfs:comment> A text representation of the depth in its original format on the specimen or in
         the collection catalogue. Example: "100 to 200 ft below sea level".</rdfs:comment>
      <rdfs:domain rdf:resource="#Specimen"/>
      <rdfs:range rdf:resource="http://www.w3.org/2001/XMLSchema#string"/>
      <rdfs:isDefinedBy rdf:resource="http://rs.tdwg.org/ontology/voc/Specimen"/>
      <tcom:darwinCoreEquivalence>Curatorial:VerbatimDepth</tcom:darwinCoreEquivalence>
   </owl:DatatypeProperty>

   <!-- Specimen::fieldNotes -->
   <owl:DatatypeProperty rdf:ID="fieldNotes">
      <rdfs:label>Field Notes</rdfs:label>
      <rdfs:comment> The text representation of field notes associated with the specimen or a link
         to those field notes.</rdfs:comment>
      <rdfs:domain rdf:resource="#Specimen"/>
      <rdfs:range rdf:resource="http://www.w3.org/2001/XMLSchema#string"/>
      <rdfs:isDefinedBy rdf:resource="http://rs.tdwg.org/ontology/voc/Specimen"/>
      <tcom:darwinCoreEquivalence>Curatorial:fieldNotes</tcom:darwinCoreEquivalence>
   </owl:DatatypeProperty>

   <!-- Specimen::lifeStage -->
   <owl:DatatypeProperty rdf:ID="lifeStage">
      <rdfs:label>Life Stage</rdfs:label>
      <rdfs:comment>The age class or life stage of the biological individual represented by the
         catalogued object. Examples: "adult", "mature", "juvenile", "eft", "nymph", "seedling",
         "seed", "egg"</rdfs:comment>
      <rdfs:domain rdf:resource="#Specimen"/>
      <rdfs:range rdf:resource="http://www.w3.org/2001/XMLSchema#string"/>
      <rdfs:isDefinedBy rdf:resource="http://rs.tdwg.org/ontology/voc/Specimen"/>
      <tcom:darwinCoreEquivalence>Core:LifeStage</tcom:darwinCoreEquivalence>
   </owl:DatatypeProperty>

   <!-- Specimen::sex -->
   <owl:DatatypeProperty rdf:ID="sex">
      <rdfs:label>Sex</rdfs:label>
      <rdfs:comment>The sex of the biological individual represented by the catalogued object.
         Examples: "male", "female", "hermaphrodite", "gynandromorph", "monoecious", "dioecious",
         "not recorded", "indeterminate", "transitional"</rdfs:comment>
      <rdfs:domain rdf:resource="#Specimen"/>
      <rdfs:range rdf:resource="http://www.w3.org/2001/XMLSchema#string"/>
      <rdfs:isDefinedBy rdf:resource="http://rs.tdwg.org/ontology/voc/Specimen"/>
      <tcom:darwinCoreEquivalence>Core:Sex</tcom:darwinCoreEquivalence>
   </owl:DatatypeProperty>


   <!-- **********************************************************************************
             K I N D    O F    S P E C I M E N    T E R M 
      ************************************************************************************-->
   <!-- KindOfSpecimenTerm -->
   <owl:Class rdf:ID="KindOfSpecimenTerm">
      <rdfs:label>Kind Of Specimen Term</rdfs:label>
      <rdfs:comment> The different kinds of Specimen. An object used to represent the different
         types of specimen.</rdfs:comment>
      <rdfs:subClassOf rdf:resource="http://rs.tdwg.org/ontology/Base#DefinedTerm"/>
      <rdfs:isDefinedBy rdf:resource="http://rs.tdwg.org/ontology/voc/Specimen"/>
   </owl:Class>
   <!-- Preserved -->
   <KindOfSpecimenTerm rdf:ID="Preserved">
      <rdfs:label>Preserved Specimen</rdfs:label>
      <dc:title>Preserved Specimen</dc:title>
      <tbase:definition>Specimen that has been preserved in some way and is intended to persist
         indefinitely. Typically a preserved specimen is also dead although this may not be the case
         with freeze dried mycological collections for example.</tbase:definition>
   </KindOfSpecimenTerm>
   <!-- Living -->
   <KindOfSpecimenTerm rdf:ID="Living">
      <rdfs:label>Living Specimen</rdfs:label>
      <dc:title>Living Specimen</dc:title>
      <tbase:definition>The specimen is alive and can be expected to change either through growth,
         reproduction and/or death.</tbase:definition>
   </KindOfSpecimenTerm>
   <!-- StillImage -->
   <KindOfSpecimenTerm rdf:ID="StillImage">
      <rdfs:label>Still Image</rdfs:label>
      <dc:title>Still Image</dc:title>
      <tbase:definition>The specimen is a picture of some kind. It may be on a physical medium or it
         may be digital.</tbase:definition>
   </KindOfSpecimenTerm>
   <!-- MovingImage -->
   <KindOfSpecimenTerm rdf:ID="MovingImage">
      <rdfs:label>Moving Image</rdfs:label>
      <dc:title>Moving Image</dc:title>
      <tbase:definition>The specimen is a moving picture of some kind. It may be on a physical
         medium or it may be digital.</tbase:definition>
   </KindOfSpecimenTerm>
   <!-- Illustration -->
   <KindOfSpecimenTerm rdf:ID="Illustration">
      <rdfs:label>Illustration Specimen</rdfs:label>
      <dc:title>Illustration Specimen</dc:title>
      <tbase:definition>The specimen is an image originally created by human hand e.g. a drawing,
         painting, etching etc.</tbase:definition>
   </KindOfSpecimenTerm>
   <!-- Digital -->
   <KindOfSpecimenTerm rdf:ID="Digital">
      <rdfs:label>Digital Specimen</rdfs:label>
      <dc:title>Digital Specimen</dc:title>
      <tbase:definition>The specimen is a digital object not a physical object.</tbase:definition>
   </KindOfSpecimenTerm>
   <!-- Fossil -->
   <KindOfSpecimenTerm rdf:ID="Fossil">
      <rdfs:label>Fossil Specimen</rdfs:label>
      <dc:title>Fossil Specimen</dc:title>
      <tbase:definition>The specimen is fossilised.</tbase:definition>
   </KindOfSpecimenTerm>

</rdf:RDF>
