<?xml version="1.0" encoding="UTF-8"?>
<!-- $Rev: 1211 $ -->
<!-- $Date: 2007-06-26 10:36:21 +0100 (Tue, 26 Jun 2007) $ -->
<!-- $Author: RogerHyam $ -->

<rdf:RDF xmlns:rdf="http://www.w3.org/1999/02/22-rdf-syntax-ns#"
   xmlns:rdfs="http://www.w3.org/2000/01/rdf-schema#" xmlns:owl="http://www.w3.org/2002/07/owl#"
   xmlns:dc="http://purl.org/dc/elements/1.1/" xmlns:dcterms="http://purl.org/dc/terms/"
   xmlns:tbase="http://rs.tdwg.org/ontology/Base#"
   xmlns:tcom="http://rs.tdwg.org/ontology/voc/Common"
   xml:base="http://rs.tdwg.org/ontology/voc/TaxonConcept"
   xmlns="http://rs.tdwg.org/ontology/voc/TaxonConcept#"
   xmlns:tc="http://rs.tdwg.org/ontology/voc/TaxonConcept#">

   <owl:Ontology rdf:about="http://rs.tdwg.org/ontology/voc/TaxonConcept">
      <dc:title>TDWG Taxon Concept LSID Ontology</dc:title>
      <dc:creator>Roger Hyam</dc:creator>
      <dc:publisher>TDWG Biodiversity Information Standards</dc:publisher>
      <dcterms:issued>2006-11-27</dcterms:issued>
      <dcterms:modified>$Date: 2007-06-26 10:36:21 +0100 (Tue, 26 Jun 2007) $</dcterms:modified>
      <dc:description>Ontology describing the metadata returned for LSIDs that are used for Taxon
         Concepts. </dc:description>

      <owl:versionInfo>0.2 - [SVN $Rev: 1211 $]</owl:versionInfo>

   </owl:Ontology>


   <!-- *****************************************
					T A X O N    C O N C E P T 
 		******************************************* -->
   <!-- TaxonConcept -->
   <owl:Class rdf:ID="TaxonConcept">
      <owl:equivalentClass rdf:resource="http://rs.tdwg.org/ontology/voc/TaxonConcept#Taxon" />
      <rdfs:label>Taxon Concept</rdfs:label>
      <rdfs:comment> Representation of a TaxonConcept. Taxon and TaxonConcept are consider equivalent.</rdfs:comment>
      <rdfs:isDefinedBy rdf:resource="http://rs.tdwg.org/ontology/voc/TaxonConcept"/>
   </owl:Class>
   
   <owl:Class rdf:ID="Taxon">
      <owl:equivalentClass rdf:resource="http://rs.tdwg.org/ontology/voc/TaxonConcept#TaxonConcept" />
      <rdfs:label>Taxon</rdfs:label>
      <rdfs:comment> Representation of a Taxon. Taxon and TaxonConcept are consider equivalent.</rdfs:comment>
      <rdfs:isDefinedBy rdf:resource="http://rs.tdwg.org/ontology/voc/TaxonConcept"/>
   </owl:Class>   

   <!-- TaxonConcept::nameString -->
   <owl:DatatypeProperty rdf:ID="nameString">
      <rdfs:label>Name String</rdfs:label>
      <rdfs:comment>A string representation of the TaxonName for this concept. Equivalent to TCS
         /DataSet/TaxonConcepts/TaxonConcept/Name/TaxonName/Simple </rdfs:comment>
      <rdfs:domain rdf:resource="#Taxon"/>
      <rdfs:isDefinedBy rdf:resource="http://rs.tdwg.org/ontology/voc/TaxonConcept"/>
   </owl:DatatypeProperty>

   <!-- TaxonConcept::hasName -->
   <owl:ObjectProperty rdf:ID="hasName">
      <rdfs:label>Has Name</rdfs:label>
      <rdfs:comment>The TaxonName for this concept. Equivalent to TCS
         /DataSet/TaxonConcepts/TaxonConcept/Name </rdfs:comment>
      <rdfs:domain rdf:resource="#Taxon"/>
      <rdfs:isDefinedBy rdf:resource="http://rs.tdwg.org/ontology/voc/TaxonConcept"/>
   </owl:ObjectProperty>

   <!-- TaxonConcept::accordingToString -->
   <owl:DatatypeProperty rdf:ID="accordingToString">
      <rdfs:label>According To String</rdfs:label>
      <rdfs:comment>A string representation of the according to for this concept. Equivalent to TCS
         /DataSet/TaxonConcepts/TaxonConcept/AccordingTo/Simple </rdfs:comment>
      <rdfs:domain rdf:resource="#Taxon"/>
      <rdfs:isDefinedBy rdf:resource="http://rs.tdwg.org/ontology/voc/TaxonConcept"/>
   </owl:DatatypeProperty>

   <!-- TaxonConcept::accordingTo -->
   <owl:ObjectProperty rdf:ID="accordingTo">
      <rdfs:label>accordingTo</rdfs:label>
      <rdfs:comment>Information about the authorship of this concept which uses the Name in their
         sense (i.e. secundum, sensu). Could be an institution or collection or team of individuals.
         Equivalent to TCS /DataSet/TaxonConcepts/TaxonConcept/AccordingTo/AccordingToDetailed </rdfs:comment>
      <rdfs:domain rdf:resource="#Taxon"/>
      <rdfs:isDefinedBy rdf:resource="http://rs.tdwg.org/ontology/voc/TaxonConcept"/>
   </owl:ObjectProperty>

   <!-- TaxonConcept::describedBy -->
   <owl:ObjectProperty rdf:ID="describedBy">
      <rdfs:label>Described By</rdfs:label>
      <rdfs:comment>A description that delimits this taxon. Equivalent to TCS
         /DataSet/TaxonConcepts/TaxonConcept/CharacterCircumscription </rdfs:comment>
      <rdfs:domain rdf:resource="#Taxon"/>
      <rdfs:isDefinedBy rdf:resource="http://rs.tdwg.org/ontology/voc/TaxonConcept"/>
   </owl:ObjectProperty>

   <!-- TaxonConcept::circumscribedBy -->
   <owl:ObjectProperty rdf:ID="circumscribedBy">
      <rdfs:label>Circumscribed By</rdfs:label>
      <rdfs:comment>A specimen that forms part of the circumscription of this taxon. Equivalent to
         TCS /DataSet/TaxonConcepts/TaxonConcept/SpecimenCircumscription </rdfs:comment>
      <rdfs:domain rdf:resource="#Taxon"/>
      <rdfs:isDefinedBy rdf:resource="http://rs.tdwg.org/ontology/voc/TaxonConcept"/>
   </owl:ObjectProperty>

   <!-- Taxonomic Hierarchy -->

   <!--is child taxon of-->
   <owl:ObjectProperty rdf:ID="isChildTaxonOf">
      <rdfs:label>Is Child Taxon Of</rdfs:label>
      <dc:title>Is Child Taxon Of</dc:title>
      <tbase:definition>Hierarchical Relationship: Concept 1 is a member of lower taxonomic rank of
         Concept 2</tbase:definition>
      <rdfs:domain rdf:resource="#Taxon"/>
      <rdfs:range rdf:resource="#Taxon"/>
      <rdfs:isDefinedBy rdf:resource="http://rs.tdwg.org/ontology/voc/TaxonConcept"/>
   </owl:ObjectProperty>

   <!--is parent taxon of-->
   <owl:ObjectProperty rdf:ID="isParentTaxonOf">
      <rdfs:label>Is Parent Taxon Of</rdfs:label>
      <dc:title>Is Parent Taxon Of</dc:title>
      <tbase:definition>Hierarchical Relationship: Taxon Concept 1 includes Concept 2 as a
         lower-ranked member.</tbase:definition>
      <rdfs:domain rdf:resource="#Taxon"/>
      <rdfs:range rdf:resource="#Taxon"/>
      <rdfs:isDefinedBy rdf:resource="http://rs.tdwg.org/ontology/voc/TaxonConcept"/>
   </owl:ObjectProperty>

   <!-- cross classification or set relationships  -->

   <!--is congruent to-->
   <owl:ObjectProperty rdf:ID="isCongruentTo">
      <rdfs:label>Is Congruent To</rdfs:label>
      <dc:title>Is Congruent To</dc:title>
      <rdfs:comment>Set Relationship: The subject and object taxa contain exactly the same set of
         individuals.</rdfs:comment>
      <rdfs:domain rdf:resource="#Taxon"/>
      <rdfs:range rdf:resource="#Taxon"/>
      <rdfs:isDefinedBy rdf:resource="http://rs.tdwg.org/ontology/voc/TaxonConcept"/>
   </owl:ObjectProperty>

   <!--includes-->
   <owl:ObjectProperty rdf:ID="includes">
      <rdfs:label>Includes</rdfs:label>
      <dc:title>Includes</dc:title>
      <rdfs:comment>Set Relationship: Every member of the object taxon is a member of the subject
         taxon.</rdfs:comment>
      <rdfs:domain rdf:resource="#Taxon"/>
      <rdfs:range rdf:resource="#Taxon"/>
      <rdfs:isDefinedBy rdf:resource="http://rs.tdwg.org/ontology/voc/TaxonConcept"/>
   </owl:ObjectProperty>

   <!--excludes-->
   <owl:ObjectProperty rdf:ID="excludes">
      <rdfs:label>Excludes</rdfs:label>
      <dc:title>Excludes</dc:title>
      <rdfs:comment>Set Relationship: No member of the object taxon is a member of the subject
         taxon.</rdfs:comment>
      <rdfs:domain rdf:resource="#Taxon"/>
      <rdfs:range rdf:resource="#Taxon"/>
      <rdfs:isDefinedBy rdf:resource="http://rs.tdwg.org/ontology/voc/TaxonConcept"/>
   </owl:ObjectProperty>

   <!--overlaps-->
   <owl:ObjectProperty rdf:ID="overlaps">
      <rdfs:label>Overlaps</rdfs:label>
      <dc:title>Overlaps</dc:title>
      <rdfs:comment> Set Relationship: The subject and object taxa have some members in common but
         both the subject and object taxa also have members they don't share.</rdfs:comment>
      <rdfs:domain rdf:resource="#Taxon"/>
      <rdfs:range rdf:resource="#Taxon"/>
      <rdfs:isDefinedBy rdf:resource="http://rs.tdwg.org/ontology/voc/TaxonConcept"/>
   </owl:ObjectProperty>

   <!-- isSynonymOf -->
   <owl:ObjectProperty rdf:ID="isSynonymOf">
      <rdfs:label>Is Synonym Of</rdfs:label>
      <dc:title>Is Synonym Of</dc:title>
      <rdfs:comment>The subject taxon is a synonym of the object taxon. This is ambiguous in terms of the set relationship.</rdfs:comment>
      <rdfs:domain rdf:resource="#Taxon"/>
      <rdfs:range rdf:resource="#Taxon"/>
      <rdfs:isDefinedBy rdf:resource="http://rs.tdwg.org/ontology/voc/TaxonConcept"/>
   </owl:ObjectProperty>

   <!--is hybrid parent of-->
   <owl:ObjectProperty rdf:ID="isHybridParentOf">
      <rdfs:label>Is Hybrid Parent Of</rdfs:label>
      <dc:title>Is Hybrid Parent Of</dc:title>
      <rdfs:comment>Hybrid Relationship: Concept 1 is genetic parent of Concept 2</rdfs:comment>
      <rdfs:domain rdf:resource="#Taxon"/>
      <rdfs:range rdf:resource="#Taxon"/>
      <rdfs:isDefinedBy rdf:resource="http://rs.tdwg.org/ontology/voc/TaxonConcept"/>
   </owl:ObjectProperty>

   <!--is male parent of-->
   <owl:ObjectProperty rdf:ID="isMaleParentOf">
      <rdfs:label>Is Male Parent Of</rdfs:label>
      <dc:title>Is Male Parent Of</dc:title>
      <rdfs:comment>Hybrid Relationship: Concept 1 is genetic father of Concept 2</rdfs:comment>
      <rdfs:domain rdf:resource="#Taxon"/>
      <rdfs:range rdf:resource="#Taxon"/>
      <rdfs:isDefinedBy rdf:resource="http://rs.tdwg.org/ontology/voc/TaxonConcept"/>
   </owl:ObjectProperty>

   <!--is female parent of-->
   <owl:ObjectProperty rdf:ID="isFemaleParentOf">
      <rdfs:label>Is Female Parent Of</rdfs:label>
      <dc:title>Is Female Parent Of</dc:title>
      <rdfs:comment>Hybrid Relationship: Concept 1 is genetic mother of Concept 2 </rdfs:comment>
      <rdfs:domain rdf:resource="#Taxon"/>
      <rdfs:range rdf:resource="#Taxon"/>
      <rdfs:isDefinedBy rdf:resource="http://rs.tdwg.org/ontology/voc/TaxonConcept"/>
   </owl:ObjectProperty>


</rdf:RDF>
