<?xml version="1.0" encoding="UTF-8"?>
<!-- $Rev: 1211 $ -->
<!-- $Date: 2007-06-26 10:36:21 +0100 (Tue, 26 Jun 2007) $ -->
<!-- $Author: RogerHyam $ -->

<rdf:RDF xmlns:rdf="http://www.w3.org/1999/02/22-rdf-syntax-ns#"
   xmlns:rdfs="http://www.w3.org/2000/01/rdf-schema#" xmlns:owl="http://www.w3.org/2002/07/owl#"
   xmlns:dc="http://purl.org/dc/elements/1.1/" xmlns:dcterms="http://purl.org/dc/terms/"
   xmlns:tbase="http://rs.tdwg.org/ontology/Base#"
   xmlns:tcom="http://rs.tdwg.org/ontology/voc/Common"
   xml:base="http://rs.tdwg.org/ontology/voc/TaxonConcept"
   xmlns="http://rs.tdwg.org/ontology/voc/TaxonConcept#"
   xmlns:tc="http://rs.tdwg.org/ontology/voc/TaxonConcept#">

   <owl:Ontology rdf:about="http://rs.tdwg.org/ontology/voc/TaxonConcept">
      <dc:title>TDWG Taxon Concept LSID Ontology</dc:title>
      <dc:creator>Roger Hyam</dc:creator>
      <dc:publisher>TDWG Biodiversity Information Standards</dc:publisher>
      <dcterms:issued>2006-11-27</dcterms:issued>
      <dcterms:modified>$Date: 2007-06-26 10:36:21 +0100 (Tue, 26 Jun 2007) $</dcterms:modified>
      <dc:description>Ontology describing the metadata returned for LSIDs that are used for Taxon
         Concepts. </dc:description>

      <owl:versionInfo>0.2 - [SVN $Rev: 1211 $]</owl:versionInfo>

      <rdfs:comment rdf:parseType="Literal"> This is not a full rendering of TaxonConcept as
         presented in the Taxon Concept Schema 1.0. Not all the possible concept-concept
         relationships have been modelled just the basic set theory and taxonomic hierarchy
         relationships. RelationshipAssertions have not been included. These omissions will be
         addressed in collaboration with the first data provider/consumer pairs who need to make use
         them. FIXME: <a href="http://phoebus.cs.man.ac.uk:9999/OWL/Validator">Wonder Web OWL
            Ontology Validator</a>
      </rdfs:comment>

   </owl:Ontology>


   <!-- *****************************************
					T A X O N    C O N C E P T 
 		******************************************* -->
   <!-- TaxonConcept -->
   <owl:Class rdf:ID="TaxonConcept">
      <rdfs:label>Taxon Concept</rdfs:label>
      <rdfs:comment> Representation of a TaxonConcept. Equivalent to TCS
         /DataSet/TaxonConcepts/TaxonConcept </rdfs:comment>
      <rdfs:subClassOf rdf:resource="http://rs.tdwg.org/ontology/Core#Concept"/>
      <rdfs:isDefinedBy rdf:resource="http://rs.tdwg.org/ontology/voc/TaxonConcept"/>
   </owl:Class>

   <!-- TaxonConcept::nameString -->
   <owl:DatatypeProperty rdf:ID="nameString">
      <rdfs:label>Name String</rdfs:label>
      <rdfs:comment>A string representation of the TaxonName for this concept. Equivalent to TCS
         /DataSet/TaxonConcepts/TaxonConcept/Name/TaxonName/Simple </rdfs:comment>
      <rdfs:domain rdf:resource="#TaxonConcept"/>
      <rdfs:range rdf:resource="http://www.w3.org/2001/XMLSchema#string"/>
      <rdfs:isDefinedBy rdf:resource="http://rs.tdwg.org/ontology/voc/TaxonConcept"/>
   </owl:DatatypeProperty>

   <!-- TaxonConcept::hasName -->
   <owl:ObjectProperty rdf:ID="hasName">
      <rdfs:label>Has Name</rdfs:label>
      <rdfs:comment>The TaxonName for this concept. Equivalent to TCS
         /DataSet/TaxonConcepts/TaxonConcept/Name </rdfs:comment>
      <rdfs:domain rdf:resource="#TaxonConcept"/>
      <rdfs:isDefinedBy rdf:resource="http://rs.tdwg.org/ontology/voc/TaxonConcept"/>
   </owl:ObjectProperty>

   <!-- TaxonConcept::accordingToString -->
   <owl:DatatypeProperty rdf:ID="accordingToString">
      <rdfs:label>According To String</rdfs:label>
      <rdfs:comment>A string representation of the according to for this concept. Equivalent to TCS
         /DataSet/TaxonConcepts/TaxonConcept/AccordingTo/Simple </rdfs:comment>
      <rdfs:domain rdf:resource="#TaxonConcept"/>
      <rdfs:isDefinedBy rdf:resource="http://rs.tdwg.org/ontology/voc/TaxonConcept"/>
   </owl:DatatypeProperty>

   <!-- TaxonConcept::accordingTo -->
   <owl:ObjectProperty rdf:ID="accordingTo">
      <rdfs:label>accordingTo</rdfs:label>
      <rdfs:comment>Information about the authorship of this concept which uses the Name in their
         sense (i.e. secundum, sensu). Could be an institution or collection or team of individuals.
         Equivalent to TCS /DataSet/TaxonConcepts/TaxonConcept/AccordingTo/AccordingToDetailed </rdfs:comment>
      <rdfs:domain rdf:resource="#TaxonConcept"/>
      <rdfs:isDefinedBy rdf:resource="http://rs.tdwg.org/ontology/voc/TaxonConcept"/>
   </owl:ObjectProperty>

   <!-- TaxonConcept::describedBy -->
   <owl:ObjectProperty rdf:ID="describedBy">
      <rdfs:label>Described By</rdfs:label>
      <rdfs:comment>A description that delimits this taxon. Equivalent to TCS
         /DataSet/TaxonConcepts/TaxonConcept/CharacterCircumscription </rdfs:comment>
      <rdfs:domain rdf:resource="#TaxonConcept"/>
      <rdfs:isDefinedBy rdf:resource="http://rs.tdwg.org/ontology/voc/TaxonConcept"/>
   </owl:ObjectProperty>

   <!-- TaxonConcept::circumscribedBy -->
   <owl:ObjectProperty rdf:ID="circumscribedBy">
      <rdfs:label>Circumscribed By</rdfs:label>
      <rdfs:comment>A specimen that forms part of the circumscription of this taxon. Equivalent to
         TCS /DataSet/TaxonConcepts/TaxonConcept/SpecimenCircumscription </rdfs:comment>
      <rdfs:domain rdf:resource="#TaxonConcept"/>
      <rdfs:isDefinedBy rdf:resource="http://rs.tdwg.org/ontology/voc/TaxonConcept"/>
   </owl:ObjectProperty>

   <!-- TaxonConcept::hasRelationship -->
   <owl:ObjectProperty rdf:ID="hasRelationship">
      <rdfs:label>hasRelationship</rdfs:label>
      <rdfs:comment>A relationship to another TaxonConcept</rdfs:comment>
      <rdfs:domain rdf:resource="#TaxonConcept"/>
      <rdfs:range rdf:resource="http://rs.tdwg.org/ontology/voc/TaxonConcept#Relationship"/>
      <rdfs:isDefinedBy rdf:resource="http://rs.tdwg.org/ontology/voc/TaxonConcept"/>
   </owl:ObjectProperty>

   <!-- TaxonConcept::rank -->
   <owl:ObjectProperty rdf:ID="rank">
      <rdfs:label>Rank</rdfs:label>
      <rdfs:comment>*Deprecated* The taxonomic rank of this concept. This is a link to an instance
         of TaxonomicRank. Compare with the rankString property. Equivalent to TCS
         /DataSet/TaxonConcepts/TaxonConcept/Rank. After discussions between a number of parties
         this property is considered to be deprecated. The rank of a TaxonConcept should be
         indicated by including a TaxonName of the appropriate rank in the hasName property even if
         the name object is empty apart from the rank.</rdfs:comment>
      <rdfs:domain rdf:resource="#TaxonConcept"/>
      <rdfs:range rdf:resource="http://rs.tdwg.org/ontology/voc/TaxonRank#TaxonRankTerm"/>
      <rdfs:isDefinedBy rdf:resource="http://rs.tdwg.org/ontology/voc/TaxonConcept"/>
      <dc:relation rdf:resource="http://rs.tdwg.org/ontology/voc/TaxonConcept#rankString"/>
   </owl:ObjectProperty>

   <!-- TaxonConcept::rankString -->
   <owl:DatatypeProperty rdf:ID="rankString">
      <rdfs:label>Rank String</rdfs:label>
      <rdfs:comment>*Deprecated* The taxonomic rank of this concept as a string. A string
         representation of the rank of this concept. It is highly recommended that the rank property
         be used along with this one unless the correct rank is not available in the rank
         vocabulary. No direct equivalent in TCS but is string version of
         /DataSet/TaxonConcepts/TaxonConcept/Rank. Requested by data suppliers. After discussions
         between a number of parties this property is considered to be deprecated. The rank of a
         TaxonConcept should be indicated by including a TaxonName of the appropriate rank in the
         hasName property even if the name object is empty apart from the rank. </rdfs:comment>
      <rdfs:domain rdf:resource="#TaxonConcept"/>
      <rdfs:range rdf:resource="http://www.w3.org/2001/XMLSchema#string"/>
      <rdfs:isDefinedBy rdf:resource="http://rs.tdwg.org/ontology/voc/TaxonConcept"/>
      <dc:relation rdf:resource="http://rs.tdwg.org/ontology/voc/TaxonConcept#rank"/>
   </owl:DatatypeProperty>

   <!-- TaxonConcept::primary -->
   <owl:DatatypeProperty rdf:ID="primary">
      <rdfs:label>Primary</rdfs:label>
      <rdfs:comment>If primary='true' the concept is the first level response to a query. If 'false'
         the concept may be a secondary concept linked directly or indirectly to the definition of a
         primary concept.</rdfs:comment>
      <rdfs:domain rdf:resource="#TaxonConcept"/>
      <rdfs:range rdf:resource="http://www.w3.org/2001/XMLSchema#boolean"/>
      <rdfs:isDefinedBy rdf:resource="http://rs.tdwg.org/ontology/voc/TaxonConcept"/>
      <dc:relation rdf:resource="http://rs.tdwg.org/ontology/voc/TaxonConcept#rank"/>
   </owl:DatatypeProperty>


   <!-- TaxonConcept::hasInformation -->
   <owl:ObjectProperty rdf:ID="hasInformation">
      <rdfs:label>Has Information</rdfs:label>
      <rdfs:comment>A piece of information about this TaxonConcept.</rdfs:comment>
      <rdfs:domain rdf:resource="#TaxonConcept"/>
      <rdfs:range rdf:resource="http://rs.tdwg.org/ontology/voc/SpeciesProfileModel#InfoItem"/>
      <rdfs:isDefinedBy rdf:resource="http://rs.tdwg.org/ontology/voc/TaxonConcept"/>
   </owl:ObjectProperty>

   <!-- Relationship -->
   <owl:Class rdf:ID="Relationship">
      <rdfs:label>Relationship</rdfs:label>
      <rdfs:comment>A typed link to with another taxon.</rdfs:comment>
      <rdfs:subClassOf rdf:resource="http://rs.tdwg.org/ontology/Base#BaseThing"/>
      <rdfs:isDefinedBy rdf:resource="http://rs.tdwg.org/ontology/voc/TaxonConcept"/>
      <tcom:tcsEquivalence>/DataSet/TaxonConcepts/TaxonConcept/Relationships/Relationship</tcom:tcsEquivalence>
   </owl:Class>

   <!-- Relationship::toTaxon -->
   <owl:ObjectProperty rdf:ID="toTaxon">
      <rdfs:label>toTaxon</rdfs:label>
      <rdfs:comment>The target taxon in this relationship.</rdfs:comment>
      <rdfs:domain rdf:resource="#Relationship"/>
      <rdfs:range rdf:resource="http://rs.tdwg.org/ontology/voc/TaxonConcept#TaxonConcept"/>
      <rdfs:isDefinedBy rdf:resource="http://rs.tdwg.org/ontology/voc/TaxonConcept"/>
      <tcom:tcsEquivalence>/DataSet/TaxonConcepts/TaxonConcept/Relationships/Relationship/ToTaxonConcept</tcom:tcsEquivalence>
   </owl:ObjectProperty>

   <!-- Relationship::fromTaxon -->
   <owl:ObjectProperty rdf:ID="fromTaxon">
      <rdfs:label>fromTaxon</rdfs:label>
      <rdfs:comment>The host taxon in this relationship.</rdfs:comment>
      <rdfs:domain rdf:resource="#Relationship"/>
      <rdfs:range rdf:resource="http://rs.tdwg.org/ontology/voc/TaxonConcept#TaxonConcept"/>
      <rdfs:isDefinedBy rdf:resource="http://rs.tdwg.org/ontology/voc/TaxonConcept"/>
      <tcom:tcsEquivalence>/DataSet/TaxonConcepts/TaxonConcept/Relationships/Relationship/FromTaxonConcept</tcom:tcsEquivalence>
   </owl:ObjectProperty>

   <!-- Relationship::relationshipCategory -->
   <owl:ObjectProperty rdf:ID="relationshipCategory">
      <rdfs:label>relationshipCategory</rdfs:label>
      <rdfs:comment>The kind of relationship this is.</rdfs:comment>
      <rdfs:domain rdf:resource="#Relationship"/>
      <rdfs:range rdf:resource="http://rs.tdwg.org/ontology/voc/TaxonConcept#TaxonRelationshipTerm"/>
      <rdfs:isDefinedBy rdf:resource="http://rs.tdwg.org/ontology/voc/TaxonConcept"/>
      <tcom:tcsEquivalence>/DataSet/TaxonConcepts/TaxonConcept/Relationships/Relationship/@type</tcom:tcsEquivalence>
   </owl:ObjectProperty>

   <!-- TaxonRelationshipTerm -->
   <owl:Class rdf:ID="TaxonRelationshipTerm">
      <rdfs:label>Taxon Relationship Term</rdfs:label>
      <rdfs:comment> The class for constructing a controlled vocabulary for TaxonConcept to
         TaxonConcept relationship categories.</rdfs:comment>
      <rdfs:subClassOf rdf:resource="http://rs.tdwg.org/ontology/Base#DefinedTerm"/>
      <rdfs:isDefinedBy rdf:resource="http://rs.tdwg.org/ontology/voc/TaxonConcept"/>
   </owl:Class>

   <!--is congruent to-->
   <TaxonRelationshipTerm rdf:ID="IsCongruentTo">
      <rdfs:label>Is Congruent To</rdfs:label>
      <dc:title>Is Congruent To</dc:title>
      <tbase:definition>Set Relationship: The extent of Concept 1 is (essentially) identical to
         Concept 2</tbase:definition>
      <tcom:tcsEquivalence>/RelationshipType/is congruent to</tcom:tcsEquivalence>
   </TaxonRelationshipTerm>

   <!--is not congruent to-->
   <TaxonRelationshipTerm rdf:ID="IsNotCongruentTo">
      <rdfs:label>Is Not Congruent To</rdfs:label>
      <dc:title>Is Not Congruent To</dc:title>
      <tbase:definition>Set Relationship: The extent of Concept 1 is not identical to Concept
         2</tbase:definition>
      <tcom:tcsEquivalence>/RelationshipType/is not congruent to</tcom:tcsEquivalence>
   </TaxonRelationshipTerm>

   <!--includes-->
   <TaxonRelationshipTerm rdf:ID="Includes">
      <rdfs:label>Includes</rdfs:label>
      <dc:title>Includes</dc:title>
      <tbase:definition>Set Relationship: Concept 2 is a subset of Concept 1</tbase:definition>
      <tcom:tcsEquivalence>/RelationshipType/includes</tcom:tcsEquivalence>
   </TaxonRelationshipTerm>

   <!--does not include-->
   <TaxonRelationshipTerm rdf:ID="DoesNotInclude">
      <rdfs:label>Does Not Include</rdfs:label>
      <dc:title>Does Not Include</dc:title>
      <tbase:definition>Set Relationship: Concept 2 is not a subset of Concept 1</tbase:definition>
      <tcom:tcsEquivalence>/RelationshipType/does not include</tcom:tcsEquivalence>
   </TaxonRelationshipTerm>

   <!--excludes-->
   <TaxonRelationshipTerm rdf:ID="Excludes">
      <rdfs:label>Excludes</rdfs:label>
      <dc:title>Excludes</dc:title>
      <tbase:definition>Set Relationship: Concept 1 does not overlap or include Concept
         2</tbase:definition>
      <tcom:tcsEquivalence>/RelationshipType/excludes</tcom:tcsEquivalence>
   </TaxonRelationshipTerm>

   <!--is included in-->
   <TaxonRelationshipTerm rdf:ID="IsIncludedIn">
      <rdfs:label>Is Included In</rdfs:label>
      <dc:title>Is Included In</dc:title>
      <tbase:definition>Set Relationship: Concept 1 is a subset of Concept 2</tbase:definition>
      <tcom:tcsEquivalence>/RelationshipType/is included in</tcom:tcsEquivalence>
   </TaxonRelationshipTerm>

   <!--is not included in-->
   <TaxonRelationshipTerm rdf:ID="IsNotIncludedIn">
      <rdfs:label>Is Not Included In</rdfs:label>
      <dc:title>Is Not Included In</dc:title>
      <tbase:definition>Set Relationship: Concept 1 is not a subset of Concept 2</tbase:definition>
      <tcom:tcsEquivalence>/RelationshipType/is not included in</tcom:tcsEquivalence>
   </TaxonRelationshipTerm>

   <!--overlaps-->
   <TaxonRelationshipTerm rdf:ID="Overlaps">
      <rdfs:label>Overlaps</rdfs:label>
      <dc:title>Overlaps</dc:title>
      <tbase:definition>Set Relationship: Concepts 1 and 2 share members/children in
         common</tbase:definition>
      <tcom:tcsEquivalence>/RelationshipType/overlaps</tcom:tcsEquivalence>
   </TaxonRelationshipTerm>

   <!--does not overlap-->
   <TaxonRelationshipTerm rdf:ID="DoesNotOverlap">
      <rdfs:label>Does Not Overlap</rdfs:label>
      <dc:title>Does Not Overlap</dc:title>
      <tbase:definition>Set Relationship: Concepts 1 and 2 have no members/children in
         common</tbase:definition>
      <tcom:tcsEquivalence>/RelationshipType/does not overlap</tcom:tcsEquivalence>
   </TaxonRelationshipTerm>

   <!--is child taxon of-->
   <TaxonRelationshipTerm rdf:ID="IsChildTaxonOf">
      <rdfs:label>Is Child Taxon Of</rdfs:label>
      <dc:title>Is Child Taxon Of</dc:title>
      <tbase:definition>Hierarchical Relationship: Concept 1 is a member of lower taxonomic rank of
         Concept 2</tbase:definition>
      <tcom:tcsEquivalence>/RelationshipType/is child taxon of</tcom:tcsEquivalence>
   </TaxonRelationshipTerm>

   <!--is parent taxon of-->
   <TaxonRelationshipTerm rdf:ID="IsParentTaxonOf">
      <rdfs:label>Is Parent Taxon Of</rdfs:label>
      <dc:title>Is Parent Taxon Of</dc:title>
      <tbase:definition>Hierarchical Relationship: Taxon Concept 1 includes Concept 2 as a
         lower-ranked member.</tbase:definition>
      <tcom:tcsEquivalence>/RelationshipType/is parent taxon of</tcom:tcsEquivalence>
   </TaxonRelationshipTerm>

   <!--is anamorph of-->
   <TaxonRelationshipTerm rdf:ID="IsAnamorphOf">
      <rdfs:label>Is Anamorph Of</rdfs:label>
      <dc:title>Is Anamorph Of</dc:title>
      <tbase:definition>Concept 1 is the asexual or mitotic reproductive stage in a pleomorphic life
         cycle in which Concept 2 is the teleomorph or meiotic reproductive stage
         .</tbase:definition>
      <tcom:tcsEquivalence>/RelationshipType/is anamorph of</tcom:tcsEquivalence>
   </TaxonRelationshipTerm>

   <!--is teleomorph of-->
   <TaxonRelationshipTerm rdf:ID="IsTeleomorphOf">
      <rdfs:label>Is Teleomorph Of</rdfs:label>
      <dc:title>Is Teleomorph Of</dc:title>
      <tbase:definition>Concept 1 is the teleomorph or meiotic reproductive stage in a pleomorphic
         life cycle in which Concept 2 is the asexual or mitotic reproductive
         stage.</tbase:definition>
      <tcom:tcsEquivalence>/RelationshipType/is teleomorph of</tcom:tcsEquivalence>
   </TaxonRelationshipTerm>

   <!--is second parent of-->
   <TaxonRelationshipTerm rdf:ID="IsSecondParentOf">
      <rdfs:label>Is Second Parent Of</rdfs:label>
      <dc:title>Is Second Parent Of</dc:title>
      <tbase:definition>Hybrid Relationship: Concept 1 is genetic parent (2) of Concept
         2.</tbase:definition>
      <tcom:tcsEquivalence>/RelationshipType/is second parent of</tcom:tcsEquivalence>
   </TaxonRelationshipTerm>

   <!--is female parent of-->
   <TaxonRelationshipTerm rdf:ID="IsFemaleParentOf">
      <rdfs:label>Is Female Parent Of</rdfs:label>
      <dc:title>Is Female Parent Of</dc:title>
      <tbase:definition>Hybrid Relationship: Concept 1 is genetic mother of Concept 2 </tbase:definition>
      <tcom:tcsEquivalence>/RelationshipType/is female parent of</tcom:tcsEquivalence>
   </TaxonRelationshipTerm>

   <!--is first parent of-->
   <TaxonRelationshipTerm rdf:ID="IsFirstParentOf">
      <rdfs:label>Is First Parent Of</rdfs:label>
      <dc:title>Is First Parent Of</dc:title>
      <tbase:definition>Hybrid Relationship: Concept 1 is genetic parent (1) of Concept
         2</tbase:definition>
      <tcom:tcsEquivalence>/RelationshipType/is first parent of</tcom:tcsEquivalence>
   </TaxonRelationshipTerm>

   <!--is male parent of-->
   <TaxonRelationshipTerm rdf:ID="IsMaleParentOf">
      <rdfs:label>Is Male Parent Of</rdfs:label>
      <dc:title>Is Male Parent Of</dc:title>
      <tbase:definition>Hybrid Relationship: Concept 1 is genetic father of Concept
         2</tbase:definition>
      <tcom:tcsEquivalence>/RelationshipType/is male parent of</tcom:tcsEquivalence>
   </TaxonRelationshipTerm>

   <!--is hybrid parent of-->
   <TaxonRelationshipTerm rdf:ID="IsHybridParentOf">
      <rdfs:label>Is Hybrid Parent Of</rdfs:label>
      <dc:title>Is Hybrid Parent Of</dc:title>
      <tbase:definition>Hybrid Relationship: Concept 1 is genetic parent of Concept
         2</tbase:definition>
      <tcom:tcsEquivalence>/RelationshipType/is hybrid parent of</tcom:tcsEquivalence>
   </TaxonRelationshipTerm>

   <!--is hybrid child of-->
   <TaxonRelationshipTerm rdf:ID="IsHybridChildOf">
      <rdfs:label>Is Hybrid Child Of</rdfs:label>
      <dc:title>Is Hybrid Child Of</dc:title>
      <tbase:definition>Hybrid Relationship: Concept 2 is a genetic parent of Concept
         1</tbase:definition>
      <tcom:tcsEquivalence>/RelationshipType/is hybrid child of</tcom:tcsEquivalence>
   </TaxonRelationshipTerm>

   <!--is ambiregnal of-->
   <TaxonRelationshipTerm rdf:ID="IsAmbiregnalOf">
      <rdfs:label>Is Ambiregnal Of</rdfs:label>
      <dc:title>Is Ambiregnal Of</dc:title>
      <tbase:definition>The two concepts are considered to represent the same taxon (i.e. they are
         congruent) but their names governed by different nomenclatural codes.</tbase:definition>
      <tcom:tcsEquivalence>/RelationshipType/is ambiregnal of (The definition is somewhat different
         as TaxonConcepts are permitted to have multiple names in the RDF version of
         TCS)</tcom:tcsEquivalence>
   </TaxonRelationshipTerm>

   <!--is vernacular for-->
   <TaxonRelationshipTerm rdf:ID="IsVernacularFor">
      <rdfs:label>Is Vernacular For</rdfs:label>
      <dc:title>Is Vernacular For</dc:title>
      <tbase:definition>The current concept is used as a vernacular concept, at least in part, for
         the target concept. This kind of relationship should not be used to express any form of set
         relationship (e.g. overlaps, is congruent with, includes). Consider using vernacular type
         relationships along with set type relationships to avoid any ambiguity.</tbase:definition>
      <tcom:tcsEquivalence>/RelationshipType/is vernacular for</tcom:tcsEquivalence>
   </TaxonRelationshipTerm>

   <!--has vernacular-->
   <TaxonRelationshipTerm rdf:ID="HasVernacular">
      <rdfs:label>Has Vernacular</rdfs:label>
      <dc:title>Has Vernacular</dc:title>
      <tbase:definition>The target concept is used as a vernacular concept, at least in part, for
         the current concept. This kind of relationship should not be used to express any form of
         set relationship (e.g. overlaps, is congruent with, includes). Consider using vernacular
         type relationships along with set type relationships to avoid any
         ambiguity.</tbase:definition>
      <tcom:tcsEquivalence>/RelationshipType/has vernacular</tcom:tcsEquivalence>
   </TaxonRelationshipTerm>

   <!--has synonym-->
   <TaxonRelationshipTerm rdf:ID="HasSynonym">
      <rdfs:label>Has Synonym</rdfs:label>
      <dc:title>Has Synonym</dc:title>
      <tbase:definition>The target concept is considered a synonym of the current concept. This is
         an ambiguous relationship. It can mean: 1) a nomenclatural relationship where all that is
         implied is that the type of the target concept is included in the current circumscription.
         This is more precisely expressed as a specimen circumscription (for heterotypic synonyms)
         or as TaxonName basionym relationships (for homotypic synonyms) 2) a concept relationship
         where some part of (or all of) the target concept is included in the current
         circumscription. This is more precisely expressed using the set relationships such as 'is
         congruent to'. The HasSynonym term is principally intended for handling legacy
         data.</tbase:definition>
      <tcom:tcsEquivalence>/RelationshipType/has synonym</tcom:tcsEquivalence>
   </TaxonRelationshipTerm>

   <!--has synonym-->
   <TaxonRelationshipTerm rdf:ID="IsSynonymFor">
      <rdfs:label>Is Synonym For</rdfs:label>
      <dc:title>Is Synonym For</dc:title>
      <tbase:definition>The current concept is considered a synonym of the target concept. This is
         an ambiguous relationship. It can mean: 1) a nomenclatural relationship where all that is
         implied is that the type of the current concept is included in the target circumscription.
         This is more precisely expressed as a specimen circumscription (for heterotypic synonyms)
         or as TaxonName basionym relationships (for homotypic synonyms) 2) a concept relationship
         where some part of (or all of) the current concept is included in the target
         circumscription. This is more precisely expressed using the set relationships such as 'is
         congruent to'. The IsSynonymFor term is principally intended for handling legacy
         data.</tbase:definition>
      <tcom:tcsEquivalence>No direct equivalent</tcom:tcsEquivalence>
   </TaxonRelationshipTerm>

</rdf:RDF>
