<?xml version="1.0"?>
<?xml-stylesheet type="text/xsl" href="human.xsl"?>
<!-- $Rev: 1294 $ -->
<!-- $Date: 2007-08-15 14:05:50 +0100 (Wed, 15 Aug 2007) $ -->
<!-- $Author: MarkusDoering $ -->
<rdf:RDF xml:base="http://rs.tdwg.org/ontology/voc/Person" xmlns="http://rs.tdwg.org/ontology/voc/Person#" xmlns:dc="http://purl.org/dc/elements/1.1/" xmlns:dcterms="http://purl.org/dc/terms/" xmlns:owl="http://www.w3.org/2002/07/owl#" xmlns:rdf="http://www.w3.org/1999/02/22-rdf-syntax-ns#" xmlns:rdfs="http://www.w3.org/2000/01/rdf-schema#" xmlns:tbase="http://rs.tdwg.org/ontology/Base#" xmlns:tp="http://rs.tdwg.org/ontology/voc/Person#">
	<owl:Ontology rdf:about="http://rs.tdwg.org/ontology/voc/Person">
		<dc:title>TDWG Person LSID Ontology</dc:title>
		<dc:creator>Roger Hyam</dc:creator>
		<dc:publisher>TDWG Biodiversity Information Standards</dc:publisher>
		<dcterms:issued>2006-11-27</dcterms:issued>
		<dcterms:modified>$Date: 2007-08-15 14:05:50 +0100 (Wed, 15 Aug 2007) $</dcterms:modified>
		<dc:description>Ontology describing the metadata returned for LSIDs that are used for People. </dc:description>
		<owl:versionInfo>0.2 - [SVN $Rev: 1294 $]</owl:versionInfo>
		<rdfs:comment rdf:parseType="Literal"> This ontology makes a basic split between people, their
         names and contact details. Note that there are no regular contact details here like
         telephone, mobile, skype name, zip code, postcode, PO Box number, Street address. The
         vocabulary does not try to represent information that is handled better by vCard or FOAF
         implementations. AACR2 rules on von, van de la and other compund names recommended.</rdfs:comment>
	</owl:Ontology>
	<!-- *****************************************
					P E R S O N 
 		******************************************* -->
	<!-- Person -->
	<owl:Class rdf:ID="Person">
		<rdfs:label>Person</rdfs:label>
		<rdfs:comment>A representation of a human being, living or dead.</rdfs:comment>
		<rdfs:subClassOf rdf:resource="http://rs.tdwg.org/ontology/Core#Person"/>
		<rdfs:isDefinedBy rdf:resource="http://rs.tdwg.org/ontology/voc/Person"/>
	</owl:Class>
	<!-- Person::lifespan -->
	<owl:DatatypeProperty rdf:ID="lifespan">
		<rdfs:label>Lifespan</rdfs:label>
		<rdfs:comment>The period for which this person was alive represented as a string. the form
         birthdate - deathdate (XXXX - YYYY; XXXX - or - YYYY as appropriate) is prefered, or as simple
         flourished date (fl. XXXX) may be given where that is all that is known. </rdfs:comment>
		<rdfs:domain rdf:resource="#Person"/>
		<rdfs:range rdf:resource="http://www.w3.org/2001/XMLSchema#string"/>
		<rdfs:isDefinedBy rdf:resource="http://rs.tdwg.org/ontology/voc/Person"/>
	</owl:DatatypeProperty>
	<!-- Person::birthdate -->
	<owl:DatatypeProperty rdf:ID="birthdate">
		<rdfs:label>Birth date</rdfs:label>
		<rdfs:comment>The date of birth of this person as an ISO date string. </rdfs:comment>
		<rdfs:domain rdf:resource="#Person"/>
		<rdfs:range rdf:resource="http://www.w3.org/2001/XMLSchema#string"/>
		<rdfs:isDefinedBy rdf:resource="http://rs.tdwg.org/ontology/voc/Person"/>
		<owl:sameAs rdf:resource="http://www.w3.org/2001/vcard-rdf/3.0#BDAY"/>
	</owl:DatatypeProperty>
	<!-- Person::deathdate -->
	<owl:DatatypeProperty rdf:ID="deathdate">
		<rdfs:label>Death date</rdfs:label>
		<rdfs:comment>The date of death of this person as an ISO date string - if appropriate.</rdfs:comment>
		<rdfs:domain rdf:resource="#Person"/>
		<rdfs:range rdf:resource="http://www.w3.org/2001/XMLSchema#string"/>
		<rdfs:isDefinedBy rdf:resource="http://rs.tdwg.org/ontology/voc/Person"/>
	</owl:DatatypeProperty>
	<!-- Person::flourishedDate -->
	<owl:DatatypeProperty rdf:ID="flourishedDate">
		<rdfs:label>Flourished date</rdfs:label>
		<rdfs:comment>A single date on which this person was known to be alive, as an ISO date string.
         If multiple dates are available then the property may be repeated.</rdfs:comment>
		<rdfs:domain rdf:resource="#Person"/>
		<rdfs:range rdf:resource="http://www.w3.org/2001/XMLSchema#string"/>
		<rdfs:isDefinedBy rdf:resource="http://rs.tdwg.org/ontology/voc/Person"/>
	</owl:DatatypeProperty>
	<!-- Person::subjectScope -->
	<owl:DatatypeProperty rdf:ID="subjectScope">
		<rdfs:label>Subject scope</rdfs:label>
		<rdfs:comment>Subject skill keyword. e.g. Entomology or Botany. May be repeated for multiple subjects.</rdfs:comment>
		<rdfs:domain rdf:resource="#Person"/>
		<rdfs:range rdf:resource="http://www.w3.org/2001/XMLSchema#string"/>
		<rdfs:isDefinedBy rdf:resource="http://rs.tdwg.org/ontology/voc/Person"/>
	</owl:DatatypeProperty>
	<!-- Person::geographicScope -->
	<owl:DatatypeProperty rdf:ID="geographicScope">
		<rdfs:label>Geographic scope</rdfs:label>
		<rdfs:comment>The geographic area this person's work was/is concerned with. e.g. 'Africa' or 'Alpine'. May be repeated for multiple areas / countries.</rdfs:comment>
		<rdfs:domain rdf:resource="#Person"/>
		<rdfs:range rdf:resource="http://www.w3.org/2001/XMLSchema#string"/>
		<rdfs:isDefinedBy rdf:resource="http://rs.tdwg.org/ontology/voc/Person"/>
	</owl:DatatypeProperty>
	<!-- Person::authorOf -->
	<owl:ObjectProperty rdf:ID="authorOf">
		<rdfs:label>Author of</rdfs:label>
		<rdfs:comment>The person has 'authored' this resource. 'Authored' here is taken in the broad
         sense. The resource may be any kind of object not just a PublicationCitation.</rdfs:comment>
		<rdfs:domain rdf:resource="#Person"/>
		<rdfs:range rdf:resource="http://rs.tdwg.org/ontology/Core#BaseThing"/>
		<rdfs:isDefinedBy rdf:resource="http://rs.tdwg.org/ontology/voc/Person"/>
	</owl:ObjectProperty>
	<!-- Person::alias -->
	<owl:ObjectProperty rdf:ID="alias">
		<rdfs:label>Alias</rdfs:label>
		<rdfs:comment>Another name this person is known by. May include nicknames, formal abbreviations or
         standard forms along with the context for use if appropriate.</rdfs:comment>
		<rdfs:domain rdf:resource="#Person"/>
		<rdfs:range rdf:resource="http://rs.tdwg.org/ontology/voc/Person#PersonNameAlias"/>
		<rdfs:isDefinedBy rdf:resource="http://rs.tdwg.org/ontology/voc/Person"/>
	</owl:ObjectProperty>
	<!-- Person::contactDetails -->
	<owl:ObjectProperty rdf:ID="contactDetails">
		<rdfs:label>Contact details</rdfs:label>
		<rdfs:comment>A link to contact information (such as postal address, email address and phone number) for this person.</rdfs:comment>
		<rdfs:domain rdf:resource="#Person"/>
		<rdfs:range rdf:resource="http://rs.tdwg.org/ontology/voc/ContactDetails#ContactDetails"/>
		<rdfs:isDefinedBy rdf:resource="http://rs.tdwg.org/ontology/voc/Person"/>
	</owl:ObjectProperty>
	<!-- *****************************************
      P E R S O N   N A M E  A L I A S 
      ******************************************* -->
	<!-- PersonNameAlias -->
	<owl:Class rdf:ID="PersonNameAlias">
		<rdfs:label>Person Name Alias</rdfs:label>
		<rdfs:comment>The respresentation of a name a person is known by and the context in which it
         should be or has been used.</rdfs:comment>
		<rdfs:subClassOf rdf:resource="http://rs.tdwg.org/ontology/Core#Name"/>
		<rdfs:isDefinedBy rdf:resource="http://rs.tdwg.org/ontology/voc/Person"/>
	</owl:Class>
	<!-- awaiting final metadata strategy 
   <owl:DatatypeProperty rdf:ID="dcAliasTitle">
      <rdfs:label>Dublin Core Title</rdfs:label>
      <rdfs:comment> Dublin Core Metadata Title for this object. 
         This property should contain a string representation of this alias in full.
         This property is represented in the TDWG Ontology as http://rs.tdwg.org/ontology/voc/Person#dcAliasTitle but it is good practise to use the Dublin Core equivalent
         http://purl.org/dc/elements/1.1/title in instance documents as it has the same meaning but it understandable to more clients. </rdfs:comment>
      <rdfs:domain rdf:resource="#PersonNameAlias"/>
      <rdfs:range rdf:resource="http://www.w3.org/2001/XMLSchema#string"/>
      <owl:sameAs rdf:resource="http://purl.org/dc/elements/1.1/title"/>
      <rdfs:isDefinedBy rdf:resource="http://rs.tdwg.org/ontology/voc/Person"/>
   </owl:DatatypeProperty>
-->
	<!-- PersonNameAlias::context -->
	<owl:DatatypeProperty rdf:ID="context">
		<rdfs:label>Context</rdfs:label>
		<rdfs:comment>The context in which this name form is used or has been used in the past. e.g.
         'Publications in German' or 'Prior to Marriage in 1964'. May include indication of formal
         standardisation system that may be represented by the ratifiedBy property. e.g. 'IPNI
         Authors'.</rdfs:comment>
		<rdfs:domain rdf:resource="#PersonNameAlias"/>
		<rdfs:range rdf:resource="http://www.w3.org/2001/XMLSchema#string"/>
		<rdfs:isDefinedBy rdf:resource="http://rs.tdwg.org/ontology/voc/Person"/>
	</owl:DatatypeProperty>
	<!-- PersonNameAlias::ratifiedBy -->
	<!-- this is removed because it replicates dc:conformsTo 
   <owl:ObjectProperty rdf:ID="ratifiedBy">
      <rdfs:label>Ratified By</rdfs:label>
      <rdfs:comment>The body that ratifies this as the correct way to cite this persons name in this
         context.</rdfs:comment>
      <rdfs:domain rdf:resource="#PersonNameAlias"/>
      <rdfs:range rdf:resource="http://rs.tdwg.org/ontology/Base#Actor"/>
      <rdfs:isDefinedBy rdf:resource="http://rs.tdwg.org/ontology/voc/Person"/>
   </owl:ObjectProperty>
   -->
	<!-- PersonNameAlias::standardForm -->
	<owl:DatatypeProperty rdf:ID="standardForm">
		<rdfs:label>Standard Form</rdfs:label>
		<rdfs:comment>The standardised, possibly abbreviated, form of the person's name in this
         context.</rdfs:comment>
		<rdfs:domain rdf:resource="#PersonNameAlias"/>
		<rdfs:range rdf:resource="http://www.w3.org/2001/XMLSchema#string"/>
		<rdfs:isDefinedBy rdf:resource="http://rs.tdwg.org/ontology/voc/Person"/>
	</owl:DatatypeProperty>
	<!-- PersonNameAlias::surname -->
	<owl:DatatypeProperty rdf:ID="surname">
		<rdfs:label>Surname</rdfs:label>
		<rdfs:comment>A hereditary name common to all members of a family, as distinct from a given
         name or forename. Where (for a double barrelled or two word name) the delimitation between
         surname and forename is not clear, name variations may be supplied with the different
         delimitations. Eg 'Tom Parker Bowles' could be handled as 'Parker Bowles, Tom' and as
         'Bowles, Tom Parker' using different PersonNameAlias objects for the same person.</rdfs:comment>
		<rdfs:domain rdf:resource="#PersonNameAlias"/>
		<rdfs:range rdf:resource="http://www.w3.org/2001/XMLSchema#string"/>
		<rdfs:isDefinedBy rdf:resource="http://rs.tdwg.org/ontology/voc/Person"/>
	</owl:DatatypeProperty>
	<!-- PersonNameAlias::forenames -->
	<owl:DatatypeProperty rdf:ID="forenames">
		<rdfs:label>Forenames</rdfs:label>
		<rdfs:comment>All other names not included in the surname. May be just initials, all forenames
         in full or a combination of expanded names and initials.</rdfs:comment>
		<rdfs:domain rdf:resource="#PersonNameAlias"/>
		<rdfs:range rdf:resource="http://www.w3.org/2001/XMLSchema#string"/>
		<rdfs:isDefinedBy rdf:resource="http://rs.tdwg.org/ontology/voc/Person"/>
	</owl:DatatypeProperty>
	<!-- PersonNameAlias::isPrefered -->
	<owl:DatatypeProperty rdf:ID="isPreferred">
		<rdfs:label>Is Preferred</rdfs:label>
		<rdfs:comment>Indicates that this is the preferred name alias for the preson.</rdfs:comment>
		<rdfs:domain rdf:resource="#PersonNameAlias"/>
		<rdfs:range rdf:resource="http://www.w3.org/2001/XMLSchema#boolean"/>
		<rdfs:isDefinedBy rdf:resource="http://rs.tdwg.org/ontology/voc/Person"/>
	</owl:DatatypeProperty>
</rdf:RDF>
